Experiments with mixed record-inductive mutual recursion
Define type, write function over this and produce good OCaml

src/core/Ty.v
@@ -1,4 +1,5 @@
 
+(*Temp*)
 Require Export Ident.
 
 
@@ -57,7 +58,6 @@ End Ty.
 
 Module TyImpl (I: Ident) <: Ty I.*)
 
-
 (*Type variables*)
 Record tvsymbol := {
   tv_name : ident
@@ -67,6 +67,921 @@ Record tvsymbol := {
 Inductive type_def (A: Set) : Set :=
   | NoDef
   | Alias: A -> type_def A.
+
+(*Unset Elimination Schemes.
+Inductive tysymbol : Set :=
+  | mk_tysymbol : ident -> list tvsymbol -> type_def ty -> tysymbol 
+with ty : Set :=
+  | mk_ty : ty_node_ -> tag -> ty
+with ty_node_ : Set :=
+  | Tyvar : tvsymbol -> ty_node_
+  | Tyapp : tysymbol -> list ty -> ty_node_.
+Set Elimination Schemes.
+
+Scheme tysymbol_ind := Induction for tysymbol Sort Prop with
+ty_ind := Induction for ty Sort Prop with
+ty_node__ind := Induction for ty_node_ Sort Prop.
+
+Check ty_ind.*)
+
+
+(*We do this to get around the restriction that
+  Coq Records and Inductives cannot be mutually recursive
+  with each other. TODO: see if we can ensure that
+  this satisfies the correct .mli file*)
+Inductive ty_ (A: Set) : Set := 
+  { ty_node: A;
+    ty_tag: tag}.
+
+Arguments ty_ {A}.
+Arguments ty_node {A}.
+Arguments ty_tag {A}.
+
+Record tysymbol_ (A: Set) : Set := {
+  ts_name : ident;
+  ts_args : list tvsymbol;
+  ts_def : type_def (@ty_ A)
+}.
+
+Arguments tysymbol_ {A}.
+Arguments ts_name {A}.
+Arguments ts_args {A}.
+Arguments ts_def {A}.
+
+Inductive ty_node_ : Set :=
+  | Tyvar : tvsymbol -> ty_node_
+  | Tyapp : @tysymbol_ ty_node_ -> list (@ty_ ty_node_) -> ty_node_.
+
+Definition ty : Set := @ty_ ty_node_.
+Definition tysymbol : Set := @tysymbol_ ty_node_.
+
+(*Test*)
+
+(*This awkward definition satisfies Coq's positivity checker
+  for nested induction, unlike the normal one*)
+Definition map2 {A B C: Type} :=
+  fun (f: A -> B -> C) =>
+    fix map2 (l1: list A) : list B -> list C :=
+      match l1 with
+      | nil => fun l2 => nil
+      | x1 :: t1 =>
+        fun l2 =>
+        match l2 with
+        | nil => nil
+        | x2 :: t2 => f x1 x2 :: map2 t1 t2
+        end
+      end.
+
+(*This doesn't work, let's try to prove induction principle*)
+Fail Fixpoint ty_equal (t1 t2: ty) {struct t1} : bool :=
+  match t1.(ty_node), t2.(ty_node) with
+  | Tyvar v1, Tyvar v2 => true
+  | Tyapp ts1 tys1, Tyapp ts2 tys2 => 
+    forallb (fun x => x) (map2 ty_equal tys1 tys2)
+  | _, _ => false
+  end.
+
+
+Definition type_def_p (P: ty -> Prop) (t: type_def ty_) : Prop :=
+  match t with
+  | NoDef _ => True
+  | Alias _ x => P x
+  end.
+
+Section TyInd.
+
+Variable (P: ty -> Prop).
+Variable (P1: ty_node_ -> Prop).
+Variable (P2: tysymbol -> Prop).
+
+Variable (Hty: forall n t, P1 n -> P (Build_ty_ _ n t)).
+Variable (Hsym: forall n vs t, type_def_p P t -> P2 (Build_tysymbol_ _ n vs t)).
+Variable (Hvar: forall v, P1 (Tyvar v)).
+Variable (Happ: forall ts tys, P2 ts -> Forall P tys -> P1 (Tyapp ts tys)).
+
+(*This does NOT work - tysymbol is not recursive so we can't have
+  a fixpoint on it
+  Maybe could do same trick (assume we have proof, populate later)
+  but likely to run into positivity problems*)
+
+Fail Fixpoint ty_ind (t: ty) : P t :=
+  match t with
+  | Build_ty_ _ n tg => Hty n tg (ty_node_ind n)
+  end
+with ty_node_ind (t: ty_node_) : P1 t :=
+  match t with
+  | Tyvar tv => Hvar tv
+  | Tyapp ts tys => Happ ts tys (tysymbol_ind ts) 
+    ((fix tys_ind (l: list ty) : Forall P l :=
+      match l with
+      | nil => List.Forall_nil _
+      | x :: xs => List.Forall_cons _ _ _ (ty_ind x) (tys_ind xs)
+      end) tys)
+  end
+with tysymbol_ind (ts: tysymbol) : P2 ts :=
+  match ts with
+  | Build_tysymbol_ _ n l d => Hsym n l d 
+    (match d as d' return type_def_p P d' with
+      | NoDef _ => I
+      | Alias _ x => ty_ind x
+    end)
+  end.
+
+End TyInd.
+
+(*Let's try bad*)
+Inductive func {A: Set} : Set :=
+  | func1: (A -> A) -> func.
+
+Fail Inductive bad : Set :=
+  | bad1: @func bad -> bad.
+
+(*Next: structural recursion on size*)
+
+(*TODO: try with Xavier trick (Equations bad extraction I think) and manual rec*)
+(*Define size*)
+Fixpoint ty_node_size (t: ty_node_) : nat :=
+  match t with
+  | Tyvar v => 1
+  | Tyapp ts tys => 1 +
+    (*tysymbol size*)
+    (1 + match (ts_def ts) with
+          | NoDef _ => 0
+          | Alias _ x => 1 + (1 + ty_node_size (x.(ty_node)))
+    end) +
+  
+   list_sum 
+      (map (fun (x: ty) => 1 + ty_node_size (x.(ty_node))) tys)
+  end.
+
+Definition ty_size (t: ty) : nat :=
+  1 + ty_node_size (t.(ty_node)).
+
+Definition tysymbol_size (ts: tysymbol) : nat :=
+  1 + match ts_def ts with
+    | NoDef _ => 0
+    | Alias _ x => 1 + ty_size x
+  end.
+
+Lemma ty_node_size_rewrite (t: ty_node_) :
+  ty_node_size t =
+  match t with
+  | Tyvar v => 1
+  | Tyapp ts tys => 1 + tysymbol_size ts + 
+    list_sum (map ty_size tys)
+  end.
+Proof.
+  destruct t; simpl; auto.
+Qed.
+
+(*Need version of map2 with in*)
+Definition map2' {A B C: Type} :=
+    fix map2 (l1: list A) : list B -> (A -> B -> C) -> list C :=
+      match l1 with
+      | nil => fun l2 f => nil
+      | x1 :: t1 =>
+        fun l2 f =>
+        match l2 with
+        | nil => nil
+        | x2 :: t2 => f x1 x2 :: map2 t1 t2 f
+        end
+      end.
+
+Definition map2'' {A B C: Type} :=
+    fix map2 (l1: list A) : forall (l2: list B), 
+      (forall (x: A) (Hinx: In x l1) (y: B) (Hiny: In y l2), C) -> list C :=
+      match l1 with
+      | nil => fun l2 f => nil
+      | x1 :: t1 =>
+        fun l2 =>
+        match l2 with
+        | nil => fun f => nil
+        | x2 :: t2 => fun f => f x1 (in_eq _ _) x2 (in_eq _ _) :: map2 t1 t2 
+          (fun x Hin y Hin2 => f x (in_cons _ _ _ Hin) y (in_cons _ _ _ Hin2))
+        end
+      end.
+
+Definition type_def_size (t: type_def ty) : nat :=
+  match t with
+  | NoDef _ => 0
+  | Alias _ x => 1 + ty_size x
+  end.
+
+
+(*Obligations (do here to test OCaml)*)
+Lemma node_lt_ty (t: ty):
+  ty_node_size (ty_node t) < ty_size t.
+Proof.
+  unfold ty_size. lia.
+Qed.
+
+Lemma ty_decomp (t: ty):
+{| ty_node := ty_node t; ty_tag := ty_tag t |} = t.
+Proof.
+  destruct t; reflexivity.
+Qed.
+
+Lemma typesym_lt_node (ts: tysymbol) (tys: list ty):
+  tysymbol_size ts < ty_node_size (Tyapp ts tys).
+Proof.
+  rewrite ty_node_size_rewrite.
+  lia.
+Qed.
+
+(*Lemma foo (x: nat) x < x + 1.
+
+Lemma bar (x y: nat) : x < y -> y > x.*)
+
+Lemma in_tys_lt_app (ts: tysymbol) (tys: list ty) :
+Forall (fun x : ty => ty_size x < ty_node_size (Tyapp ts tys)) tys.
+Proof.
+  (*TODO: bad proof*)
+  rewrite ty_node_size_rewrite.
+  rewrite List.Forall_forall; intros x Hinx.
+  pose proof (in_split x tys Hinx) as Hsplit.
+  destruct Hsplit as [l1 [l2 Htys]]; subst.
+  rewrite map_app; simpl.
+  rewrite list_sum_app. simpl. unfold ty_size at 1. lia.
+Qed.
+
+Lemma alias_lt_sym {x ts}:
+type_def_size (Alias ty_ x) < tysymbol_size ts ->
+ty_size x < tysymbol_size ts.
+Proof.
+  simpl. lia.
+Qed.
+
+Lemma def_lt_sym ts: type_def_size (ts_def ts) < tysymbol_size ts.
+Proof.
+  unfold tysymbol_size; simpl.
+  destruct (ts_def ts); auto.
+Qed.
+
+(*Let's try to prove an induction principle*)
+
+Section TyInd.
+
+Variable (P: ty -> Prop).
+Variable (P1: ty_node_ -> Prop).
+Variable (P2: tysymbol -> Prop).
+
+Variable (Hty: forall (t: ty), P1 (t.(ty_node)) -> P t).
+Variable (Hsym: forall (ts: tysymbol), type_def_p P (ts.(ts_def)) ->
+  P2 ts).
+Variable (Hvar: forall v, P1 (Tyvar v)).
+Variable (Happ: forall ts tys, P2 ts -> Forall P tys -> P1 (Tyapp ts tys)).
+
+(*This does NOT work - tysymbol is not recursive so we can't have
+  a fixpoint on it
+  Maybe could do same trick (assume we have proof, populate later)
+  but likely to run into positivity problems*)
+
+
+(*Fixpoint gcd_rec (a b: nat) (ACC: Acc lt b) {struct ACC} : nat :=
+  if Nat.eq_dec b 0 then a else gcd_rec b (a mod b) (Acc_inv ACC _).*)
+
+(*TODO: need decomposition if we want idiomatic code, maybe need eq_rect*)
+(*Plan: prove lemmas, do in Set, test extraction (without Program) *)
+Fixpoint ty_ind' (t: ty) (ACC: Acc lt (ty_size t)) {struct ACC} : P t :=
+  (Hty t (ty_node_ind' t.(ty_node) 
+    (Acc_inv ACC (ty_node_size (ty_node t)) (node_lt_ty t))))
+with ty_node_ind' (t: ty_node_) (ACC: Acc lt (ty_node_size t)) {struct ACC} : P1 t :=
+  match t as t' return Acc lt (ty_node_size t') -> P1 t' with
+  | Tyvar tv => fun _ => Hvar tv
+  | Tyapp ts tys => fun ACC => Happ ts tys (tysymbol_ind' ts (Acc_inv ACC (tysymbol_size ts) 
+      (typesym_lt_node ts tys))) 
+    ((fix tys_ind (l: list ty) 
+      (Hl: Forall (fun x => ty_size x < (ty_node_size (Tyapp ts tys))) l) 
+      : Forall P l :=
+      match l as l' return Forall  (fun x => ty_size x < (ty_node_size (Tyapp ts tys))) l'->
+        Forall P l'  with
+      | nil => fun _ => List.Forall_nil _
+      | x :: xs => fun Hl => List.Forall_cons _ _ _ (ty_ind' x (Acc_inv ACC (ty_size x) 
+        (List.Forall_inv Hl))) 
+        (tys_ind xs (List.Forall_inv_tail Hl))
+      end Hl) tys (in_tys_lt_app ts tys))
+  end ACC
+with tysymbol_ind' (ts: tysymbol) (ACC: Acc lt (tysymbol_size ts)) {struct ACC} : P2 ts :=
+  Hsym ts (
+    match (ts.(ts_def)) as d' return type_def_size d' < tysymbol_size ts -> 
+       type_def_p P d' with
+    | NoDef _ => fun _ => I
+    | Alias _ x => fun Hlt => ty_ind' x (Acc_inv ACC (ty_size x) (alias_lt_sym Hlt))
+    end (def_lt_sym ts)
+  ).
+
+Definition ty_ind (t: ty) : P t := ty_ind' t (lt_wf _).
+Definition ty_node_ind (t: ty_node_) : P1 t := ty_node_ind' t (lt_wf _).
+Definition tysymbol_ind (ts: tysymbol) : P2 ts := tysymbol_ind' ts (lt_wf _).
+
+End TyInd.
+
+(*Do same with Type so that we can write functions and test extraction*)
+
+Definition type_def_p_ty (P: ty -> Type) (t: type_def ty_) : Type :=
+  match t with
+  | NoDef _ => True
+  | Alias _ x => P x
+  end.
+
+
+Inductive ForallT {A: Type} (P: A -> Type) : list A -> Type :=
+  | ForallT_nil: ForallT P nil
+  | ForallT_cons: forall {x: A} {l: list A},
+    P x -> ForallT P l -> ForallT P (x :: l).
+
+Lemma ForallT_hd {A: Type} (P: A -> Type) (x: A) (l: list A):
+  ForallT P (x :: l) ->
+  P x.
+Proof.
+  intros. inversion X; subst. apply X0.
+Qed.
+
+Lemma ForallT_tl {A: Type} (P: A -> Type) (x: A) (l: list A):
+  ForallT P (x :: l) ->
+  ForallT P l.
+Proof.
+  intros. inversion X; auto.
+Qed.
+
+Lemma ForallT_In {A: Type} (P: A -> Type)
+  (eq_dec: forall (x y: A), {x = y} + {x <> y}) (l: list A):
+  ForallT P l ->
+  forall x, In x l -> P x.
+Proof.
+  intros Hall. induction Hall; simpl; intros.
+  destruct H.
+  destruct (eq_dec x x0); subst; auto.
+  apply IHHall. destruct H; subst; auto.
+  contradiction.
+Qed.
+
+Section TyRect.
+
+Variable (P: ty -> Type).
+Variable (P1: ty_node_ -> Type).
+Variable (P2: tysymbol -> Type).
+
+Variable (Hty: forall (t: ty), P1 (t.(ty_node)) -> P t).
+Variable (Hsym: forall (ts: tysymbol), type_def_p_ty P (ts.(ts_def)) ->
+  P2 ts).
+Variable (Hvar: forall v, P1 (Tyvar v)).
+Variable (Happ: forall ts tys, P2 ts -> ForallT P tys -> P1 (Tyapp ts tys)).
+
+(*This does NOT work - tysymbol is not recursive so we can't have
+  a fixpoint on it
+  Maybe could do same trick (assume we have proof, populate later)
+  but likely to run into positivity problems*)
+
+
+(*Fixpoint gcd_rec (a b: nat) (ACC: Acc lt b) {struct ACC} : nat :=
+  if Nat.eq_dec b 0 then a else gcd_rec b (a mod b) (Acc_inv ACC _).*)
+
+(*TODO: need decomposition if we want idiomatic code, maybe need eq_rect*)
+(*Plan: prove lemmas, do in Set, test extraction (without Program) *)
+Fixpoint ty_rect' (t: ty) (ACC: Acc lt (ty_size t)) {struct ACC} : P t :=
+  (Hty t (ty_node_rect' t.(ty_node) 
+    (Acc_inv ACC (ty_node_size (ty_node t)) (node_lt_ty t))))
+with ty_node_rect' (t: ty_node_) (ACC: Acc lt (ty_node_size t)) {struct ACC} : P1 t :=
+  match t as t' return Acc lt (ty_node_size t') -> P1 t' with
+  | Tyvar tv => fun _ => Hvar tv
+  | Tyapp ts tys => fun ACC => Happ ts tys (tysymbol_rect' ts (Acc_inv ACC (tysymbol_size ts) 
+      (typesym_lt_node ts tys))) 
+    ((fix tys_rect (l: list ty) 
+      (Hl: Forall (fun x => ty_size x < (ty_node_size (Tyapp ts tys))) l) 
+      : ForallT P l :=
+      match l as l' return Forall  (fun x => ty_size x < (ty_node_size (Tyapp ts tys))) l'->
+        ForallT P l'  with
+      | nil => fun _ => ForallT_nil _
+      | x :: xs => fun Hl => ForallT_cons _ (ty_rect' x (Acc_inv ACC (ty_size x) 
+        (List.Forall_inv Hl))) 
+        (tys_rect xs (List.Forall_inv_tail Hl))
+      end Hl) tys (in_tys_lt_app ts tys))
+  end ACC
+with tysymbol_rect' (ts: tysymbol) (ACC: Acc lt (tysymbol_size ts)) {struct ACC} : P2 ts :=
+  Hsym ts (
+    match (ts.(ts_def)) as d' return type_def_size d' < tysymbol_size ts -> 
+       type_def_p_ty P d' with
+    | NoDef _ => fun _ => I
+    | Alias _ x => fun Hlt => ty_rect' x (Acc_inv ACC (ty_size x) (alias_lt_sym Hlt))
+    end (def_lt_sym ts)
+  ).
+
+Definition ty_rect (t: ty) : P t := ty_rect' t (lt_wf _).
+Definition ty_node_rect (t: ty_node_) : P1 t := ty_node_rect' t (lt_wf _).
+Definition tysymbol_rect (ts: tysymbol) : P2 ts := tysymbol_rect' ts (lt_wf _).
+
+End TyRect.
+
+(*Alternate version, more useful*)
+Section TyBuild.
+
+(*First is for ty, second is for ty_node_*)
+Variable (A: Type) (B: Type) (C: Type).
+
+(*type, result of calling function on t.ty_node, result*)
+Variable (Hty: ty -> B -> A).
+Variable (Hvar: tvsymbol -> B).
+(*TODO: not general enough probably*)
+(*3rd param: folding over the resulting list*)
+Variable (base: C).
+Variable (combine: C -> A -> C).
+(*B is result of fold over list of tys*)
+Variable (Happ: tysymbol -> list ty -> C -> B).
+
+Fixpoint ty_build' (t: ty) (ACC: Acc lt (ty_size t)) {struct ACC} : A :=
+  (Hty t (ty_node_build' t.(ty_node)
+    (Acc_inv ACC (ty_node_size (ty_node t)) (node_lt_ty t))))
+with ty_node_build' (t: ty_node_) (ACC: Acc lt (ty_node_size t)) {struct ACC} : B :=
+  match t as t' return Acc lt (ty_node_size t') -> B with
+  | Tyvar tv => fun _ => Hvar tv
+  | Tyapp ts tys => fun ACC => Happ ts tys
+    (*Here, we implement fold*)
+    ((fix tys_fold (l: list ty) 
+      (Hl: Forall (fun x => ty_size x < (ty_node_size (Tyapp ts tys))) l) 
+      : C :=
+      match l as l' return Forall  (fun x => ty_size x < (ty_node_size (Tyapp ts tys))) l'->
+        C  with
+      | nil => fun _ => base
+      | x :: xs => fun Hl => combine (tys_fold xs (List.Forall_inv_tail Hl))
+          (ty_build' x (Acc_inv ACC (ty_size x) 
+        (List.Forall_inv Hl)))
+      end Hl) tys (in_tys_lt_app ts tys))
+  end ACC.
+
+Definition ty_build (t: ty) := ty_build' t (lt_wf _).
+Definition ty_node_build (t: ty_node_) := ty_node_build' t (lt_wf _).
+
+(*Hmm instead should do*)
+Definition ty_size_rel (t1 t2: ty) : Prop :=
+  ty_size t1 < ty_size t2.
+
+Require Import Coq.Wellfounded.Inverse_Image.
+
+Lemma ty_size_rel_wf: well_founded ty_size_rel.
+Proof.
+  unfold wf. intros.
+  unfold ty_size_rel.
+  apply Inverse_Image.Acc_inverse_image.
+  apply lt_wf.
+Qed.
+
+End TyBuild.
+
+Lemma in_tys_lt_app' {t ts tys}:
+  ty_node_size (Tyapp ts tys) < ty_size t ->
+  Forall (fun x => ty_size_rel x t) tys.
+Proof.
+  rewrite ty_node_size_rewrite. intros.
+  intros.
+  rewrite List.Forall_forall; intros x Hinx.
+  unfold ty_size_rel.
+  pose proof (in_split x tys Hinx) as Hsplit.
+  destruct Hsplit as [l1 [l2 Htys]]; subst.
+  revert H.
+  rewrite map_app. simpl map.
+  rewrite list_sum_app. simpl list_sum.
+  intros.
+  unfold ty_size at 1. lia.
+Qed.
+  
+Section TyBuildSimpl.
+
+Variable (A: Type)(B: Type).
+
+Variable (Hvar: tvsymbol -> A).
+Variable (Happ: tysymbol -> list ty -> B -> A).
+
+Variable (base: B).
+Variable (combine: A -> B -> B).
+
+Fixpoint ty_build_simpl' (t: ty) (ACC: Acc ty_size_rel t) {struct ACC} : A :=
+  match t.(ty_node) as n return ty_node_size n < ty_size t -> A with
+  | Tyvar v => fun _ => Hvar v
+  | Tyapp ts tys => fun Hlt => Happ ts tys
+    ((fix tys_fold (l: list ty) (Hall: Forall (fun x => ty_size_rel x t) l) : B :=
+      match l as l' return Forall (fun x => ty_size_rel x t) l' -> B with
+      | nil => fun _ => base
+      | x :: xs => fun Hall => 
+        combine (ty_build_simpl' x (Acc_inv ACC _ (Forall_inv Hall))) 
+        (tys_fold xs (Forall_inv_tail Hall))
+      end Hall) tys (in_tys_lt_app'  Hlt))
+  end (node_lt_ty t).
+
+Definition ty_build_simpl t := ty_build_simpl' t (ty_size_rel_wf t).
+
+(*This is what we need*)
+Definition ty_node_size_rel (t1 t2: ty) : Prop :=
+  ty_node_size (t1.(ty_node)) < ty_node_size (t2.(ty_node)).
+
+Lemma ty_node_size_rel_wf: well_founded ty_node_size_rel.
+Proof.
+  unfold wf. intros.
+  unfold ty_node_size_rel.
+  apply Inverse_Image.Acc_inverse_image.
+  apply lt_wf.
+Qed.
+
+Lemma ty_size_rel_node_rel (t1 t2: ty):
+  ty_size_rel t1 t2 <-> ty_node_size_rel t1 t2.
+Proof.
+  unfold ty_size_rel, ty_size, ty_node_size_rel. lia.
+Qed.
+
+
+Lemma ty_build_simpl_irrel t ACC1 ACC2:
+  ty_build_simpl' t ACC1 = ty_build_simpl' t ACC2.
+Proof.
+  induction t using (well_founded_induction ty_node_size_rel_wf).
+  destruct ACC1; destruct ACC2.
+  simpl.
+  destruct t as [n tg]; simpl. destruct n; auto.
+  f_equal.
+  generalize dependent (in_tys_lt_app' (node_lt_ty {| ty_node := Tyapp t l; ty_tag := tg |})).
+  (*assert (ty_size {| ty_node := Tyapp t l; ty_tag := tg |} <= )*)
+  generalize dependent {| ty_node := Tyapp t l; ty_tag := tg |}.
+  induction l; simpl; auto.
+  intros. erewrite IHl. f_equal.
+  apply H.
+  inversion f; subst.
+  apply ty_size_rel_node_rel. auto.
+  auto.
+Qed.
+
+
+
+
+
+Lemma ty_build_simpl_rewrite (t: ty) :
+  ty_build_simpl t =
+  match t.(ty_node) with
+        | Tyvar v => Hvar v
+        | Tyapp ts tys => Happ ts tys 
+            (fold_right (fun x acc => combine (ty_build_simpl x) acc) base tys)
+  end.
+Proof.
+  unfold ty_build_simpl at 1.
+  generalize dependent (ty_size_rel_wf t).
+  intros a. destruct a.
+  destruct t as [n tg].
+  destruct n; [reflexivity |].
+  simpl. f_equal.
+  (*Problem: have l in Forall*)
+  generalize dependent (in_tys_lt_app' (node_lt_ty {| ty_node := Tyapp t l; ty_tag := tg |})).
+  (*assert (ty_size {| ty_node := Tyapp t l; ty_tag := tg |} <= )*)
+  generalize dependent {| ty_node := Tyapp t l; ty_tag := tg |}.
+  intros t' a'.
+  (*TODO: see if we need size info*)
+  induction l; simpl; auto.
+  intros.
+  rewrite IHl.
+  f_equal.
+  apply ty_build_simpl_irrel.
+Qed.
+
+End TyBuildSimpl.
+
+
+
+(*TODO: prove this later*)
+(*Ltac hide_right := match goal with |- _ = ?rhs =>remember rhs end. 
+
+Lemma ty_build_rewrite (t: ty):
+  ty_build t =
+  Hty t (match t.(ty_node) with
+        | Tyvar v => Hvar v
+        | Tyapp ts tys => Happ ts tys 
+            (fold_right (fun x acc => combine acc (ty_build x)) base tys)
+  end).
+Proof.
+  unfold ty_build.
+  destruct (lt_wf (ty_size t)) as [a].
+  simpl ty_build' at 1. f_equal.
+  generalize dependent (a (ty_node_size (ty_node t)) (node_lt_ty t)).
+  intros a1.
+  destruct a1. 
+  
+
+  
+   unfold ty_node_build'. cbv beta. cbv. simpl ty_node_build' at 1.
+  destruct t as [n tg].
+  destruct n.
+  - simpl; auto.
+  - hide_right. simpl. subst b.
+    simpl ty_node. cbv iota. f_equal.
+    generalize dependent (in_tys_lt_app t l).
+    induction l; auto.
+    intros Hall. (*TODO: bad hack*) Opaque ty_build'. simpl.
+    f_equal.
+    erewrite <- IHl.
+
+    Unshelve. reflexivity.
+    f_equal.
+
+
+    + auto.
+    + simpl. auto.
+
+
+
+
+  
+  
+   simpl ty_node_build' at 1.
+  destruct t as [n tg].
+  simpl ty_node at 1 2 .
+  simpl.
+
+
+  (*To generalize*)
+  assert (forall (f: forall x : ty_, Acc lt (ty_node_size (ty_node x))),
+    Hty t (ty_node_build' (ty_node t) (a (ty_node_size (ty_node t)) (node_lt_ty t))) =
+    match ty_node t with
+    | 
+
+
+
+
+  generalize dependent (fun x => (Acc_intro (ty_node_size (ty_node x)) (λ (b : nat) (Hb : b < ty_node_size (ty_node x)), nat_ind (λ n : nat, ∀ a0 : nat, a0 < n → Acc (ltof nat (λ m : nat, m)) a0) (λ (a0 : nat) (Ha : a0 < 0), False_ind (Acc (ltof nat (λ m : nat, m)) a0) (PeanoNat.Nat.nlt_0_r a0 Ha)) (λ (n : nat) (IHn : ∀ a0 : nat, a0 < n → Acc (ltof nat (λ m : nat, m)) a0) (a0 : nat) (Ha : a0 < S n), Acc_intro a0 (λ (b0 : nat) (Hb0 : b0 < a0), IHn b0 (PeanoNat.Nat.lt_le_trans b0 a0 n Hb0 (match PeanoNat.Nat.succ_le_mono a0 n with
+| conj _ H0 => H0
+end Ha)))) (ty_node_size (ty_node x)) b (PeanoNat.Nat.lt_le_trans b (ty_node_size (ty_node x)) (ty_node_size (ty_node x)) Hb (match PeanoNat.Nat.succ_le_mono (ty_node_size (ty_node x)) (ty_node_size (ty_node x)) with
+| conj _ H0 => H0
+end (PeanoNat.Nat.lt_le_trans (ty_node_size (ty_node x)) (ty_size x) (ty_size x) (node_lt_ty x) (match PeanoNat.Nat.succ_le_mono (ty_size x) (ty_size x) with
+| conj _ H0 => H0
+end (PeanoNat.Nat.lt_succ_diag_r (ty_size x))))))))).
+
+
+  generalize dependent 
+  Check Acc_intro.
+  match goal with
+  | |- context [Acc_intro ?a ?b ?c ?d] => idtac a
+  end.
+  generalize dependent (a (ty_node_size (ty_node t)) (node_lt_ty t)).
+  destruct t; simpl. intros a1. f_equal.
+  destruct ty_node0; simpl.
+  - destruct a1; auto.
+  - destruct a1; simpl. f_equal.
+  
+  
+   destruct (a 1 (node_lt_ty {| ty_node := Tyvar t; ty_tag := ty_tag0 |})); simpl; auto.
+  - destruct ((a (S (S (match ts_def t with
+| NoDef _ => 0
+| Alias _ x => S (S (ty_node_size (ty_node x)))
+end + list_sum (map (λ x : ty, S (ty_node_size (ty_node x))) l)))))).
+  
+   unfold ty_node_build'; simpl.
+
+  (*generalize dependent (lt_wf (ty_size t)).*)
+  induction t using (well_founded_induction (ty_size_rel_wf)).
+  intros ACC.
+  destruct t as [n tg].
+  inversion ACC.
+  unfold ty_build' at 1. simpl.
+  simpl ty_build'. at 1.
+  simpl at 1.
+  destruct t; simpl in *.
+
+
+
+  revert t.
+  eapply ty_ind with (P1).
+  - intros.
+
+    destruct t0; simpl.
+  
+   with (P:= fun t => forall(a : Acc lt (ty_size t)), ty_build' t a = Hty t match ty_node t with
+| Tyvar v => Hvar v
+| Tyapp ts tys => Happ ts tys (foldr (λ (x : ty) (acc : C), combine acc (ty_build' x (lt_wf (ty_size x)))) base tys)
+end ).
+
+  dependent induction (ty_size t) using (well_founded_induction lt_wf).
+  unfold ty_build'. simpl. 
+        
+        
+        
+        combine base tys))
+
+
+End TyBuild.*)
+
+Definition ty_v_map (f: tvsymbol -> ty) (t: ty) : ty :=
+  ty_build_simpl ty (list ty) (fun v => f v)
+  (fun ts tys res => Build_ty_ _ (Tyapp ts res) xH) 
+  nil cons t.
+
+Definition ty_v_map' (f: tvsymbol -> ty) (t: ty) : ty :=
+  ty_build ty ty (list ty) (fun _ x => x) (fun v => f v)
+  nil (fun acc x => x :: acc) (fun ts tys res => 
+    Build_ty_ _ (Tyapp ts res) xH) t.
+
+
+(*
+Definition ty_v_map (f: tvsymbol -> ty) (t: ty) :=
+  ty_build ty (fun _ x => x) (fun v => f v) (fun ts tys IHl =>
+    Build_ty_ _ (Tyapp ts IHl) xH).
+
+
+Eval compute in 
+
+(*Let us do ty_v_map first*)
+Definition ty_v_map (f: tvsymbol -> ty) (t: ty) :=
+  ty_rect (fun (_: ty) => ty) (fun (_: ty_node) => ty) (fun _ => unit)
+  (*ty case*)
+  (fun (t1: ty) (res: bool) => res)
+  (fun _ _ => tt)
+  (*Tvar*)
+  (fun (v: tvsymbol) => f v)
+  (*Tyapp*)
+  (fun (ts: tysymbol) (tys: list ty) (IH))
+
+(*Common pattern:
+  let rec ty_foo (t1 t2: ty) : A :=
+    match t1.ty_node, t2.ty_node with
+    | *)
+
+(*Test*)
+Fixpoint list_eq (l1 l2: list nat) : bool :=
+  match l1, l2 with
+  | x1 :: t1, x2 :: t2 => Nat.eqb x1 x2 && list_eq t1 t2
+  | nil, nil => true
+  | _, _ => false
+  end.
+
+Definition list_eq' (l1 l2: list nat) : bool.
+revert l2.
+induction l1 as [| x1 t1 eq_t1]; intros l2.
+- destruct l2.
+  + apply true.
+  + apply false.
+- destruct l2 as [| x2 t2].
+  + apply false.
+  + apply (Nat.eqb x1 x2 && eq_t1 t2).
+Defined.
+
+Definition list_eq'' : list nat -> list nat -> bool :=
+  (list_rec (fun (_ : list nat) => list nat -> bool)
+    (*nil case*)
+    (fun l2 => match l2 with
+              | nil => true
+              | _ => false
+    end)
+    (*cons case*)
+    (fun x1 t1 (IH: list nat -> bool) (l2: list nat) =>
+      match l2 with
+      | nil => false
+      | x2 :: t2 => Nat.eqb x1 x2 && IH t2
+      end
+    )).
+(*NOTE: I think we DONT want ForallT, maybe want fixpoint instead but see*)
+(*NOTE: want version without tysymbol*)
+(*Now we can define an equality function (maybe)*)
+Definition ty_equal (t1 t2: ty) : bool :=
+  ty_rect (fun (_: ty) => ty -> bool ) (fun (_: ty_node_ ) => ty_node_ -> bool) 
+    (fun _ => unit)
+  (*ty case*)
+  (fun (t1: ty) (node_eq: ty_node_ -> bool) (t2: ty) =>
+    node_eq (t2.(ty_node))
+  )
+  (*tysymbol case*)
+  (fun (ts1: tysymbol) _ => tt)
+  (*ty_node_ Tyvar case*)
+  (fun (v1: tvsymbol) (t2: ty_node_) =>
+    match t2 with
+    | Tyvar v2 => true (*TODO*)
+    | _ => false
+    end) 
+  (*ty_node_ Tyapp case*)
+  (fun (ts: tysymbol) (tys: list ty) (_: unit) IH (t2: ty_node_) =>
+    match t2 with
+    | Tyvar v2 => false
+    | Tyapp ts2 tys2 => IH tys2 (*nope*)
+    end)
+  
+  .
+
+
+
+
+
+
+  ty_rect (fun _ => ty -> bool) (fun _ => ty_node_ -> bool) (fun _ => unit) t1.
+
+
+
+
+
+
+Next Obligation.
+intros. subst. unfold ty_size. simpl. apply Nat.lt_succ_diag_r.
+Qed.
+Next Obligation.
+intros. subst. rewrite ty_node_size_rewrite.
+(*bad*) lia.
+Qed.
+Next Obligation.
+intros. subst. apply Forall_inv in Hl. assumption.
+Defined.
+Next Obligation.
+intros.
+subst. apply Forall_inv_tail in Hl; assumption.
+Defined.
+Next Obligation.
+intros.
+rewrite List.Forall_forall.
+(*Not great proof*)
+clear; intros.
+rewrite ty_node_size_rewrite.
+pose proof (in_split x tys H).
+destruct H0 as [l1 [l2 Htys]]; subst.
+rewrite map_app; simpl.
+rewrite list_sum_app. simpl. unfold ty_size at 1. lia.
+Qed.
+Next Obligation.
+intros. subst.
+simpl in Hlt. lia.
+Qed.
+Next Obligation.
+intros. subst. unfold tysymbol_size. simpl.
+destruct d; simpl; auto.
+Qed.
+
+
+Record tysymbol_ (A: Set) : Set := {
+  ts_name : ident;
+  ts_args : list tvsymbol;
+  ts_def : type_def (@ty_ A)
+}.
+ 
+
+Search In
+rewrite Forall_forall.
+intros.
+
+clear. induction tys; simpl; auto.
+constructor; auto.
+- 
+
+
+subst.
+
+
+ Search Forall. rewrite ty_node_size_rewrite.
+
+ simpl.
+
+ Search (?x < S ?x). 
+
+
+End TyInd.
+
+(*Now can we do proof on Acc?*)
+Fixpoint ty_equal (t1 t2: ty) (ACC: Acc lt (ty_size t1)) {struct ACC} : bool :=
+  match t1.(ty_node), t2.(ty_node) with
+  | Tyvar v1, Tyvar v2 => true
+  | Tyapp ts1 tys1, Tyapp ts2 tys2 => 
+    forallb (fun x => x) (map2'' tys1 tys2
+      (fun x Hinx y Hiny => ty_equal x y (Acc_inv _ _ _)))
+  | _, _ => false
+  end.
+
+
+  do 3 f_equal.
+  induction l; simpl; auto.
+  rewrite IHl. reflexivity.
+  f_equal. f_equal. f_equal.
+  unfold ty_node_size.
+    (1 + match (ts_def ts) with
+          | NoDef _ => 0
+          | Alias _ x => 1 + (1 + ty_node_size (x.(ty_node)))
+    end) +
+  
+   fold_right plus 0 
+      (map (fun (x: ty) => ty_node_size (x.(ty_node))) tys)
+  end.
+
+Print tysymbol_.
+
+Definition ty_size {A: Type} (sz: A -> nat)
+
+
+
+
+Definition ty_size {A: Type} (sz: A -> nat) (t: @ty_ A) : nat :=
+
+
+
+
+
+Print tysymbol_.
+
+
+Print ty_.
+
+Print ty_node_.
+
+Variable ()
+    
+
 
 (*Fail Inductive tysymbol := {
   ts_name : I.ident;
@@ -84,7 +999,7 @@ with ty_node_ :=
 
 (*1 version:
 *)
-Inductive tysymbol : Set :=
+(*Inductive tysymbol : Set :=
   | mk_tysymbol : ident -> list tvsymbol -> type_def ty -> tysymbol 
 with ty : Set :=
   | mk_ty : ty_node_ -> tag -> ty
@@ -115,15 +1030,15 @@ Definition ty_node (t: ty) : ty_node_ :=
 Definition ty_tag (t: ty) : tag :=
   match t with
   | mk_ty _ t => t
-  end.
+  end.*)
   
 (*ts_equal and ty_equal are reference equality in OCaml impl*)
 Definition ts_equal (t1 t2: tysymbol) : bool :=
-  id_equal (ts_name t1) (ts_name t2).
+  id_equal (ts_name _ t1) (ts_name _ t2).
 
 (*End TyImpl.*)
 
-
+*)
 
 
 
