extract/Extract.v
@@ -8,5 +8,10 @@ Extract Inductive bool => "bool" [ "true" "false" ].
 Extract Inductive list => "list" [ "[]" "(::)" ].
 Extract Inductive option => "option" [ "None" "Some" ].
 Extract Inductive unit => "unit" [ "()" ].
-Separate Extraction Ident Ty.
+Extraction Inline ty_build.
+Extraction Inline ty_build'.
+Extraction Inline ty_build_simpl.
+Extraction Inline ty_build_simpl'.
+Separate Extraction Ty.ty Ty.ty_v_map Ident.
+
 (*Recursive Extraction Library Ty.*)
